src/FLeXFuncSelf.v
@@ -1,0 +1,437 @@
+Require Import Coq.Program.Basics. 
+Require Import Coq.Strings.String. 
+Require Import Coq.Logic.FunctionalExtensionality. 
+Require Import Coq.Program.Combinators. 
+Require Import Coq.Unicode.Utf8. 
+Require Import Coq.Program.Equality.
+Require Import Coq.Logic.ProofIrrelevance.
+Require Import List.
+Import ListNotations.
+
+
+Local Open Scope program_scope. 
+
+Require Import FinProof.Common. 
+Require Import FinProof.ProgrammingWith. 
+Require Import FinProof.StateMonad21. 
+Require Import FinProof.EpsilonMonad.
+Require Import FinProof.StateMonad21Instances.
+Require Import FinProof.MonadTransformers21.
+
+Require Import UMLang.SolidityNotations2.
+Require Import UMLang.ProofEnvironment2.
+
+Require Import FLeXContractTypes.
+Require Import FLeXClassSelf.
+Require Import FLeXConstSig.  
+Require Import ZArith.
+Require Import FLeXFuncNotations.
+Require Import UMLang.SolidityNotations2.
+Require Import UMLang.SML_NG25.
+
+Module FLeXFuncs (dc : FLeXConstsTypesSig XTypesModule StateMonadModule ).
+ 
+Module Export FLeXFuncNotationsModule := FLeXFuncNotations XTypesModule StateMonadModule dc.
+Import UrsusNotations.
+Local Open Scope ursus_scope.
+Local Open Scope struct_scope.
+Local Open Scope Z_scope.
+
+
+(* Existing Instance xint_default. *)
+(* Existing Instance xbool_default. *)
+(* Existing Instance true_default. *)
+Instance TvmCell_default : XDefault (TvmCell) := {
+default := xStrNull}.
+Existing Instance TvmCell_default.
+Existing Instance phantom_default .
+
+
+
+Definition FLeX_Ф_constructor ( deployer_pubkey : XInteger256 ) ( transfer_tip3 : XInteger128 ) ( return_ownership : XInteger128 ) ( trading_pair_deploy : XInteger128 ) ( order_answer : XInteger128 ) ( process_queue : XInteger128 ) ( send_notify : XInteger128 ) ( min_amount : XInteger128 ) ( deals_limit : XInteger8 ) ( notify_addr : XAddress ) : UExpression PhantomType false . 
+ 	 	 refine {{ deployer_pubkey : ( XInteger256 ) @ "deployer_pubkey" ; { _ } }} . 
+ 	 	 refine {{ transfer_tip3 : ( XInteger128 ) @ "transfer_tip3" ; { _ } }} . 
+ 	 	 refine {{ return_ownership : ( XInteger128 ) @ "return_ownership" ; { _ } }} . 
+ 	 	 refine {{ trading_pair_deploy : ( XInteger128 ) @ "trading_pair_deploy" ; { _ } }} . 
+ 	 	 refine {{ order_answer : ( XInteger128 ) @ "order_answer" ; { _ } }} . 
+ 	 	 refine {{ process_queue : ( XInteger128 ) @ "process_queue" ; { _ } }} . 
+ 	 	 refine {{ send_notify : ( XInteger128 ) @ "send_notify" ; { _ } }} . 
+ 	 	 refine {{ min_amount : ( XInteger128 ) @ "min_amount" ; { _ } }} . 
+ 	 	 refine {{ deals_limit : ( XInteger8 ) @ "deals_limit" ; { _ } }} . 
+ 	 	 refine {{ notify_addr : ( XAddress ) @ "notify_addr" ; { _ } }} . 
+ 	 	 refine {{ FLeX.deployer_pubkey_ := !{ deployer_pubkey } ; { _ } }} . 
+ 	 	 refine {{ FLeX.min_amount_ := !{ min_amount } ; { _ } }} . 
+ 	 	 refine {{ FLeX.deals_limit_ := !{ deals_limit } ; { _ } }} . 
+ 	 	 refine {{ FLeX.notify_addr_ := !{ notify_addr } ; { _ } }} . 
+ 	 	 refine {{ FLeX.tons_cfg_ := {} (* { !{ transfer_tip3 } , !{ return_ownership } , !{ trading_pair_deploy } , !{ order_answer } , !{ process_queue } , !{ send_notify } }  *) }} . 
+ Defined . 
+ 
+ (*begin*) 
+ Definition FLeX_Ф_constructor_call  ( deployer_pubkey : URValue XInteger256 false ) ( transfer_tip3 : URValue XInteger128 false ) ( return_ownership : URValue XInteger128 false ) ( trading_pair_deploy : URValue XInteger128 false ) ( order_answer : URValue XInteger128 false ) ( process_queue : URValue XInteger128 false ) ( send_notify : URValue XInteger128 false ) ( min_amount : URValue XInteger128 false ) ( deals_limit : URValue XInteger8 false ) ( notify_addr : URValue XAddress false ) := 
+ 🏓 ursus_call_with_args ( LedgerableWithArgs := λ10 ) FLeX_Ф_constructor 
+ ( SimpleLedgerableArg URValue {{ Λ "deployer_pubkey" }} deployer_pubkey ) 
+ ( SimpleLedgerableArg URValue {{ Λ "transfer_tip3" }} transfer_tip3 ) 
+ ( SimpleLedgerableArg URValue {{ Λ "return_ownership" }} return_ownership ) 
+ ( SimpleLedgerableArg URValue {{ Λ "trading_pair_deploy" }} trading_pair_deploy ) 
+ ( SimpleLedgerableArg URValue {{ Λ "order_answer" }} order_answer ) 
+ ( SimpleLedgerableArg URValue {{ Λ "process_queue" }} process_queue ) 
+ ( SimpleLedgerableArg URValue {{ Λ "send_notify" }} send_notify ) 
+ ( SimpleLedgerableArg URValue {{ Λ "min_amount" }} min_amount ) 
+ ( SimpleLedgerableArg URValue {{ Λ "deals_limit" }} deals_limit ) 
+ ( SimpleLedgerableArg URValue {{ Λ "notify_addr" }} notify_addr ) 
+ . 
+ Notation " 'FLeX_Ф_constructor_ref_' '(' deployer_pubkey transfer_tip3 return_ownership trading_pair_deploy order_answer process_queue send_notify min_amount deals_limit notify_addr ')' " := 
+ ( URResult ( FLeX_Ф_constructor_call 
+ deployer_pubkey transfer_tip3 return_ownership trading_pair_deploy order_answer process_queue send_notify min_amount deals_limit notify_addr )) 
+ (in custom URValue at level 0 , deployer_pubkey custom URValue at level 0 
+ , transfer_tip3 custom ULValue at level 0 
+ , return_ownership custom ULValue at level 0 
+ , trading_pair_deploy custom ULValue at level 0 
+ , order_answer custom ULValue at level 0 
+ , process_queue custom ULValue at level 0 
+ , send_notify custom ULValue at level 0 
+ , min_amount custom ULValue at level 0 
+ , deals_limit custom ULValue at level 0 
+ , notify_addr custom ULValue at level 0 ) : ursus_scope . 
+ (*end*) 
+ 
+ (* Definition FLeX_Ф_isFullyInitialized : UExpression XBool false . 
+ 	 	 refine {{ return_ !{pair_code_} && !{price_code_} && xchg_pair_code_ && xchg_price_code_ ; { _ } }} . 
+ Defined . 
+ 
+ (*begin*) 
+ Definition FLeX_Ф_isFullyInitialized_call  := 
+ 🏓 ursus_call_with_args ( LedgerableWithArgs := λ0 ) FLeX_Ф_isFullyInitialized 
+ . 
+ Notation " 'FLeX_Ф_isFullyInitialized_ref_' '(' ')' " := 
+ ( URResult ( FLeX_Ф_isFullyInitialized_call 
+ )) 
+ (in custom URValue at level 0 ) : ursus_scope . 
+ (*end*) 
+ 
+ Definition FLeX_Ф_setPairCode ( code : TvmCell ) : UExpression PhantomType true . 
+ 	 	 refine {{ code : ( TvmCell ) @ "code" ; { _ } }} . 
+ 	 	 refine {{ require ( ( ! isFullyInitialized ( ) . get ( ) ) , error_code::cant_override_code ) ; { _ } }} . 
+ 	 	 refine {{ require ( ( msg_pubkey ( ) == FLeX.deployer_pubkey_ ) , error_code::sender_is_not_deployer ) ; { _ } }} . 
+ 	 	 refine {{ tvm_accept ( ) ; { _ } }} . 
+ 	 	 refine {{ require ( ( ! FLeX.pair_code_ ) , error_code::cant_override_code ) ; { _ } }} . 
+ 	 	 refine {{ require ( ( code ^^ TvmCell:ctos ( ) . srefs ( ) == 2 ) , error_code::unexpected_refs_count_in_code ) ; { _ } }} . 
+ 	 	 refine {{ FLeX.pair_code_ := builder ( ) . stslice ( !{ code } . ctos ( ) ) . stref ( build ( Address { tvm_myaddr ( ) } ) . endc ( ) ) . endc ( ) ; { _ } }} . 
+ Defined . 
+ 
+ (*begin*) 
+ Definition FLeX_Ф_setPairCode_call  ( code : URValue TvmCell false ) := 
+ 🏓 ursus_call_with_args ( LedgerableWithArgs := λ1 ) FLeX_Ф_setPairCode 
+ ( SimpleLedgerableArg URValue {{ Λ "code" }} code ) 
+ . 
+ Notation " 'FLeX_Ф_setPairCode_ref_' '(' code ')' " := 
+ ( URResult ( FLeX_Ф_setPairCode_call 
+ code )) 
+ (in custom URValue at level 0 , code custom URValue at level 0 ) : ursus_scope . 
+ (*end*) 
+ 
+ Definition FLeX_Ф_setXchgPairCode ( code : TvmCell ) : UExpression PhantomType true . 
+ 	 	 refine {{ code : ( TvmCell ) @ "code" ; { _ } }} . 
+ 	 	 refine {{ require ( ( ! isFullyInitialized ( ) . get ( ) ) , error_code::cant_override_code ) ; { _ } }} . 
+ 	 	 refine {{ require ( ( msg_pubkey ( ) == FLeX.deployer_pubkey_ ) , error_code::sender_is_not_deployer ) ; { _ } }} . 
+ 	 	 refine {{ tvm_accept ( ) ; { _ } }} . 
+ 	 	 refine {{ require ( ( ! FLeX.xchg_pair_code_ ) , error_code::cant_override_code ) ; { _ } }} . 
+ 	 	 refine {{ require ( ( code ^^ TvmCell:ctos ( ) . srefs ( ) == 2 ) , error_code::unexpected_refs_count_in_code ) ; { _ } }} . 
+ 	 	 refine {{ FLeX.xchg_pair_code_ := builder ( ) . stslice ( !{ code } . ctos ( ) ) . stref ( build ( Address { tvm_myaddr ( ) } ) . endc ( ) ) . endc ( ) ; { _ } }} . 
+ Defined . 
+ 
+ (*begin*) 
+ Definition FLeX_Ф_setXchgPairCode_call  ( code : URValue TvmCell false ) := 
+ 🏓 ursus_call_with_args ( LedgerableWithArgs := λ1 ) FLeX_Ф_setXchgPairCode 
+ ( SimpleLedgerableArg URValue {{ Λ "code" }} code ) 
+ . 
+ Notation " 'FLeX_Ф_setXchgPairCode_ref_' '(' code ')' " := 
+ ( URResult ( FLeX_Ф_setXchgPairCode_call 
+ code )) 
+ (in custom URValue at level 0 , code custom URValue at level 0 ) : ursus_scope . 
+ (*end*) 
+ 
+ Definition FLeX_Ф_setPriceCode ( code : TvmCell ) : UExpression PhantomType true . 
+ 	 	 refine {{ code : ( TvmCell ) @ "code" ; { _ } }} . 
+ 	 	 refine {{ require ( ( ! isFullyInitialized ( ) . get ( ) ) , error_code::cant_override_code ) ; { _ } }} . 
+ 	 	 refine {{ require ( ( msg_pubkey ( ) == FLeX.deployer_pubkey_ ) , error_code::sender_is_not_deployer ) ; { _ } }} . 
+ 	 	 refine {{ tvm_accept ( ) ; { _ } }} . 
+ 	 	 refine {{ require ( ( ! FLeX.price_code_ ) , error_code::cant_override_code ) ; { _ } }} . 
+ 	 	 refine {{ FLeX.price_code_ := !{ code } ; { _ } }} . 
+ Defined . 
+ 
+ (*begin*) 
+ Definition FLeX_Ф_setPriceCode_call  ( code : URValue TvmCell false ) := 
+ 🏓 ursus_call_with_args ( LedgerableWithArgs := λ1 ) FLeX_Ф_setPriceCode 
+ ( SimpleLedgerableArg URValue {{ Λ "code" }} code ) 
+ . 
+ Notation " 'FLeX_Ф_setPriceCode_ref_' '(' code ')' " := 
+ ( URResult ( FLeX_Ф_setPriceCode_call 
+ code )) 
+ (in custom URValue at level 0 , code custom URValue at level 0 ) : ursus_scope . 
+ (*end*) 
+ 
+ Definition FLeX_Ф_setXchgPriceCode ( code : TvmCell ) : UExpression PhantomType true . 
+ 	 	 refine {{ code : ( TvmCell ) @ "code" ; { _ } }} . 
+ 	 	 refine {{ require ( ( ! isFullyInitialized ( ) . get ( ) ) , error_code::cant_override_code ) ; { _ } }} . 
+ 	 	 refine {{ require ( ( msg_pubkey ( ) == FLeX.deployer_pubkey_ ) , error_code::sender_is_not_deployer ) ; { _ } }} . 
+ 	 	 refine {{ tvm_accept ( ) ; { _ } }} . 
+ 	 	 refine {{ require ( ( ! FLeX.xchg_price_code_ ) , error_code::cant_override_code ) ; { _ } }} . 
+ 	 	 refine {{ FLeX.xchg_price_code_ := !{ code } ; { _ } }} . 
+ Defined . 
+ 
+ (*begin*) 
+ Definition FLeX_Ф_setXchgPriceCode_call  ( code : URValue TvmCell false ) := 
+ 🏓 ursus_call_with_args ( LedgerableWithArgs := λ1 ) FLeX_Ф_setXchgPriceCode 
+ ( SimpleLedgerableArg URValue {{ Λ "code" }} code ) 
+ . 
+ Notation " 'FLeX_Ф_setXchgPriceCode_ref_' '(' code ')' " := 
+ ( URResult ( FLeX_Ф_setXchgPriceCode_call 
+ code )) 
+ (in custom URValue at level 0 , code custom URValue at level 0 ) : ursus_scope . 
+ (*end*) 
+ 
+ Definition FLeX_Ф_getTonsCfg : UExpression TonsConfig false . 
+ 	 	 refine {{ return_ FLeX.tons_cfg_ ; { _ } }} . 
+ Defined . 
+ 
+ (*begin*) 
+ Definition FLeX_Ф_getTonsCfg_call  := 
+ 🏓 ursus_call_with_args ( LedgerableWithArgs := λ0 ) FLeX_Ф_getTonsCfg 
+ . 
+ Notation " 'FLeX_Ф_getTonsCfg_ref_' '(' ')' " := 
+ ( URResult ( FLeX_Ф_getTonsCfg_call 
+ )) 
+ (in custom URValue at level 0 ) : ursus_scope . 
+ (*end*) 
+ 
+ Definition FLeX_Ф_getTradingPairCode : UExpression TvmCell false . 
+ 	 	 refine {{ return_ *pair_code_ ; { _ } }} . 
+ Defined . 
+ 
+ (*begin*) 
+ Definition FLeX_Ф_getTradingPairCode_call  := 
+ 🏓 ursus_call_with_args ( LedgerableWithArgs := λ0 ) FLeX_Ф_getTradingPairCode 
+ . 
+ Notation " 'FLeX_Ф_getTradingPairCode_ref_' '(' ')' " := 
+ ( URResult ( FLeX_Ф_getTradingPairCode_call 
+ )) 
+ (in custom URValue at level 0 ) : ursus_scope . 
+ (*end*) 
+ 
+ Definition FLeX_Ф_getXchgPairCode : UExpression TvmCell false . 
+ 	 	 refine {{ return_ *xchg_pair_code_ ; { _ } }} . 
+ Defined . 
+ 
+ (*begin*) 
+ Definition FLeX_Ф_getXchgPairCode_call  := 
+ 🏓 ursus_call_with_args ( LedgerableWithArgs := λ0 ) FLeX_Ф_getXchgPairCode 
+ . 
+ Notation " 'FLeX_Ф_getXchgPairCode_ref_' '(' ')' " := 
+ ( URResult ( FLeX_Ф_getXchgPairCode_call 
+ )) 
+ (in custom URValue at level 0 ) : ursus_scope . 
+ (*end*) 
+ 
+ Definition FLeX_Ф_getSellPriceCode ( tip3_addr : XAddress ) : UExpression TvmCell true . 
+ 	 	 refine {{ tip3_addr : ( XAddress ) @ "tip3_addr" ; { _ } }} . 
+ 	 	 refine {{ require ( ( FLeX.price_code_ - > ctos ( ) . srefs ( ) == 2 ) , error_code::unexpected_refs_count_in_code ) ; { _ } }} . 
+ 	 	 refine {{ salt : ( TvmCell ) @ "salt" ; { _ } }} . 
+ 	 	 refine {{ { salt } := builder ( ) . stslice ( tvm_myaddr ( ) ) . stslice ( !{ tip3_addr } . sl ( ) ) . endc ( ) ; { _ } }} . 
+ 	 	 refine {{ return_ builder ( ) . stslice ( FLeX.price_code_ - > ctos ( ) ) . stref ( !{ salt } ) . endc ( ) ; { _ } }} . 
+ Defined . 
+ 
+ (*begin*) 
+ Definition FLeX_Ф_getSellPriceCode_call  ( tip3_addr : URValue XAddress false ) := 
+ 🏓 ursus_call_with_args ( LedgerableWithArgs := λ1 ) FLeX_Ф_getSellPriceCode 
+ ( SimpleLedgerableArg URValue {{ Λ "tip3_addr" }} tip3_addr ) 
+ . 
+ Notation " 'FLeX_Ф_getSellPriceCode_ref_' '(' tip3_addr ')' " := 
+ ( URResult ( FLeX_Ф_getSellPriceCode_call 
+ tip3_addr )) 
+ (in custom URValue at level 0 , tip3_addr custom URValue at level 0 ) : ursus_scope . 
+ (*end*) 
+ 
+ Definition FLeX_Ф_getXchgPriceCode ( tip3_addr1 : XAddress ) ( tip3_addr2 : XAddress ) : UExpression TvmCell true . 
+ 	 	 refine {{ tip3_addr1 : ( XAddress ) @ "tip3_addr1" ; { _ } }} . 
+ 	 	 refine {{ tip3_addr2 : ( XAddress ) @ "tip3_addr2" ; { _ } }} . 
+ 	 	 refine {{ require ( ( FLeX.price_code_ - > ctos ( ) . srefs ( ) == 2 ) , error_code::unexpected_refs_count_in_code ) ; { _ } }} . 
+ 	 	 refine {{ keys : ( auto ) @ "keys" ; { _ } }} . 
+ 	 	 refine {{ { keys } := std : : make_tuple ( !{ tip3_addr1 } , !{ tip3_addr2 } ) ; { _ } }} . 
+ 	 	 refine {{ return_ builder ( ) . stslice ( FLeX.xchg_price_code_ - > ctos ( ) ) . stref ( build ( !{ keys } ) . endc ( ) ) . endc ( ) ; { _ } }} . 
+ Defined . 
+ 
+ (*begin*) 
+ Definition FLeX_Ф_getXchgPriceCode_call  ( tip3_addr1 : URValue XAddress false ) ( tip3_addr2 : URValue XAddress false ) := 
+ 🏓 ursus_call_with_args ( LedgerableWithArgs := λ2 ) FLeX_Ф_getXchgPriceCode 
+ ( SimpleLedgerableArg URValue {{ Λ "tip3_addr1" }} tip3_addr1 ) 
+ ( SimpleLedgerableArg URValue {{ Λ "tip3_addr2" }} tip3_addr2 ) 
+ . 
+ Notation " 'FLeX_Ф_getXchgPriceCode_ref_' '(' tip3_addr1 tip3_addr2 ')' " := 
+ ( URResult ( FLeX_Ф_getXchgPriceCode_call 
+ tip3_addr1 tip3_addr2 )) 
+ (in custom URValue at level 0 , tip3_addr1 custom URValue at level 0 
+ , tip3_addr2 custom ULValue at level 0 ) : ursus_scope . 
+ (*end*) 
+ 
+ Definition Ф_prepare_trading_pair_state_init_and_addr ( pair_data : DTradingPair ) ( pair_code : TvmCell ) : UExpression ( StateInit # XInteger256 ) false . 
+ 	 	 refine {{ pair_data : ( DTradingPair ) @ "pair_data" ; { _ } }} . 
+ 	 	 refine {{ pair_code : ( TvmCell ) @ "pair_code" ; { _ } }} . 
+ 	 	 refine {{ pair_data_cl : ( TvmCell ) @ "pair_data_cl" ; { _ } }} . 
+ 	 	 refine {{ { pair_data_cl } := prepare_persistent_data ( { } , pair_data ) ; { _ } }} . 
+ 	 	 refine {{ pair_init : ( StateInitP ) @ "pair_init" ; { _ } }} . 
+ 	 	 refine {{ { pair_init } := new { { } , { } , pair_code , pair_data_cl , { } } ; { _ } }} . 
+ 	 	 refine {{ pair_init_cl : ( TvmCell ) @ "pair_init_cl" ; { _ } }} . 
+ 	 	 refine {{ { pair_init_cl } := build ( !{ pair_init } ) . make_cell ( ) ; { _ } }} . 
+ 	 	 refine {{ return_ [ !{ pair_init } , tvm_hash ( pair_init_cl ) ] ; { _ } }} . 
+ Defined . 
+ 
+ (*begin*) 
+ Definition Ф_prepare_trading_pair_state_init_and_addr_call  ( pair_data : URValue DTradingPairP false ) ( pair_code : URValue TvmCell false ) := 
+ 🏓 ursus_call_with_args ( LedgerableWithArgs := λ2 ) Ф_prepare_trading_pair_state_init_and_addr 
+ ( SimpleLedgerableArg URValue {{ Λ "pair_data" }} pair_data ) 
+ ( SimpleLedgerableArg URValue {{ Λ "pair_code" }} pair_code ) 
+ . 
+ Notation " 'Ф_prepare_trading_pair_state_init_and_addr_ref_' '(' pair_data pair_code ')' " := 
+ ( URResult ( Ф_prepare_trading_pair_state_init_and_addr_call 
+ pair_data pair_code )) 
+ (in custom URValue at level 0 , pair_data custom URValue at level 0 
+ , pair_code custom ULValue at level 0 ) : ursus_scope . 
+ (*end*) 
+ 
+ Definition FLeX_Ф_getSellTradingPair ( tip3_root : XAddress ) : UExpression XAddress false . 
+ 	 	 refine {{ tip3_root : ( XAddress ) @ "tip3_root" ; { _ } }} . 
+ 	 	 refine {{ myaddr : ( XAddress ) @ "myaddr" ; { _ } }} . 
+ 	 	 refine {{ { myaddr } := new { tvm_myaddr ( ) } ; { _ } }} . 
+ 	 	 refine {{ pair_data : ( DTradingPairP ) @ "pair_data" ; { _ } }} . 
+ 	 	 refine {{ { pair_data } := new { . flex_addr_ = myaddr , . tip3_root_ = tip3_root , . deploy_value_ = tons_cfg_ . trading_pair_deploy } ; { _ } }} . 
+ 	 	 refine {{ std_addr : ( auto ) @ "std_addr" ; { _ } }} . 
+ 	 	 refine {{ { std_addr } := prepare_trading_pair_state_init_and_addr ( !{ pair_data } , *pair_code_ ) . second ; { _ } }} . 
+ 	 	 refine {{ workchain_id : ( auto ) @ "workchain_id" ; { _ } }} . 
+ 	 	 refine {{ { workchain_id } := Std :: get < addr_std > ( !{ myaddr } . Val ( ) ) . workchain_id ; { _ } }} . 
+ 	 	 refine {{ return_ Address :: make_std ( !{ workchain_id } , !{ std_addr } ) ; { _ } }} . 
+ Defined . 
+ 
+ (*begin*) 
+ Definition FLeX_Ф_getSellTradingPair_call  ( tip3_root : URValue XAddress false ) := 
+ 🏓 ursus_call_with_args ( LedgerableWithArgs := λ1 ) FLeX_Ф_getSellTradingPair 
+ ( SimpleLedgerableArg URValue {{ Λ "tip3_root" }} tip3_root ) 
+ . 
+ Notation " 'FLeX_Ф_getSellTradingPair_ref_' '(' tip3_root ')' " := 
+ ( URResult ( FLeX_Ф_getSellTradingPair_call 
+ tip3_root )) 
+ (in custom URValue at level 0 , tip3_root custom URValue at level 0 ) : ursus_scope . 
+ (*end*) 
+ 
+ Definition Ф_prepare_xchg_pair_state_init_and_addr ( pair_data : DXchgPair ) ( pair_code : TvmCell ) : UExpression ( StateInit # XInteger256 ) false . 
+ 	 	 refine {{ pair_data : ( DXchgPair ) @ "pair_data" ; { _ } }} . 
+ 	 	 refine {{ pair_code : ( TvmCell ) @ "pair_code" ; { _ } }} . 
+ 	 	 refine {{ pair_data_cl : ( TvmCell ) @ "pair_data_cl" ; { _ } }} . 
+ 	 	 refine {{ { pair_data_cl } := prepare_persistent_data ( { } , pair_data ) ; { _ } }} . 
+ 	 	 refine {{ pair_init : ( StateInitP ) @ "pair_init" ; { _ } }} . 
+ 	 	 refine {{ { pair_init } := new { { } , { } , pair_code , pair_data_cl , { } } ; { _ } }} . 
+ 	 	 refine {{ pair_init_cl : ( TvmCell ) @ "pair_init_cl" ; { _ } }} . 
+ 	 	 refine {{ { pair_init_cl } := build ( !{ pair_init } ) . make_cell ( ) ; { _ } }} . 
+ 	 	 refine {{ return_ [ !{ pair_init } , tvm_hash ( pair_init_cl ) ] ; { _ } }} . 
+ Defined . 
+ 
+ (*begin*) 
+ Definition Ф_prepare_xchg_pair_state_init_and_addr_call  ( pair_data : URValue DXchgPairP false ) ( pair_code : URValue TvmCell false ) := 
+ 🏓 ursus_call_with_args ( LedgerableWithArgs := λ2 ) Ф_prepare_xchg_pair_state_init_and_addr 
+ ( SimpleLedgerableArg URValue {{ Λ "pair_data" }} pair_data ) 
+ ( SimpleLedgerableArg URValue {{ Λ "pair_code" }} pair_code ) 
+ . 
+ Notation " 'Ф_prepare_xchg_pair_state_init_and_addr_ref_' '(' pair_data pair_code ')' " := 
+ ( URResult ( Ф_prepare_xchg_pair_state_init_and_addr_call 
+ pair_data pair_code )) 
+ (in custom URValue at level 0 , pair_data custom URValue at level 0 
+ , pair_code custom ULValue at level 0 ) : ursus_scope . 
+ (*end*) 
+ 
+ Definition FLeX_Ф_getXchgTradingPair ( tip3_major_root : XAddress ) ( tip3_minor_root : XAddress ) : UExpression XAddress false . 
+ 	 	 refine {{ tip3_major_root : ( XAddress ) @ "tip3_major_root" ; { _ } }} . 
+ 	 	 refine {{ tip3_minor_root : ( XAddress ) @ "tip3_minor_root" ; { _ } }} . 
+ 	 	 refine {{ myaddr : ( XAddress ) @ "myaddr" ; { _ } }} . 
+ 	 	 refine {{ { myaddr } := new { tvm_myaddr ( ) } ; { _ } }} . 
+ 	 	 refine {{ pair_data : ( DXchgPairP ) @ "pair_data" ; { _ } }} . 
+ 	 	 refine {{ { pair_data } := new { . flex_addr_ = myaddr , . tip3_major_root_ = tip3_major_root , . tip3_minor_root_ = tip3_minor_root , . deploy_value_ = tons_cfg_ . trading_pair_deploy } ; { _ } }} . 
+ 	 	 refine {{ std_addr : ( auto ) @ "std_addr" ; { _ } }} . 
+ 	 	 refine {{ { std_addr } := prepare_xchg_pair_state_init_and_addr ( !{ pair_data } , *xchg_pair_code_ ) . second ; { _ } }} . 
+ 	 	 refine {{ workchain_id : ( auto ) @ "workchain_id" ; { _ } }} . 
+ 	 	 refine {{ { workchain_id } := Std :: get < addr_std > ( !{ myaddr } . Val ( ) ) . workchain_id ; { _ } }} . 
+ 	 	 refine {{ return_ Address :: make_std ( !{ workchain_id } , !{ std_addr } ) ; { _ } }} . 
+ Defined . 
+ 
+ (*begin*) 
+ Definition FLeX_Ф_getXchgTradingPair_call  ( tip3_major_root : URValue XAddress false ) ( tip3_minor_root : URValue XAddress false ) := 
+ 🏓 ursus_call_with_args ( LedgerableWithArgs := λ2 ) FLeX_Ф_getXchgTradingPair 
+ ( SimpleLedgerableArg URValue {{ Λ "tip3_major_root" }} tip3_major_root ) 
+ ( SimpleLedgerableArg URValue {{ Λ "tip3_minor_root" }} tip3_minor_root ) 
+ . 
+ Notation " 'FLeX_Ф_getXchgTradingPair_ref_' '(' tip3_major_root tip3_minor_root ')' " := 
+ ( URResult ( FLeX_Ф_getXchgTradingPair_call 
+ tip3_major_root tip3_minor_root )) 
+ (in custom URValue at level 0 , tip3_major_root custom URValue at level 0 
+ , tip3_minor_root custom ULValue at level 0 ) : ursus_scope . 
+ (*end*) 
+ 
+ Definition FLeX_Ф_getMinAmount : UExpression XInteger128 false . 
+ 	 	 refine {{ return_ FLeX.min_amount_ ; { _ } }} . 
+ Defined . 
+ 
+ (*begin*) 
+ Definition FLeX_Ф_getMinAmount_call  := 
+ 🏓 ursus_call_with_args ( LedgerableWithArgs := λ0 ) FLeX_Ф_getMinAmount 
+ . 
+ Notation " 'FLeX_Ф_getMinAmount_ref_' '(' ')' " := 
+ ( URResult ( FLeX_Ф_getMinAmount_call 
+ )) 
+ (in custom URValue at level 0 ) : ursus_scope . 
+ (*end*) 
+ 
+ Definition FLeX_Ф_getDealsLimit : UExpression XInteger8 false . 
+ 	 	 refine {{ return_ FLeX.deals_limit_ ; { _ } }} . 
+ Defined . 
+ 
+ (*begin*) 
+ Definition FLeX_Ф_getDealsLimit_call  := 
+ 🏓 ursus_call_with_args ( LedgerableWithArgs := λ0 ) FLeX_Ф_getDealsLimit 
+ . 
+ Notation " 'FLeX_Ф_getDealsLimit_ref_' '(' ')' " := 
+ ( URResult ( FLeX_Ф_getDealsLimit_call 
+ )) 
+ (in custom URValue at level 0 ) : ursus_scope . 
+ (*end*) 
+ 
+ Definition FLeX_Ф_getNotifyAddr : UExpression XAddress false . 
+ 	 	 refine {{ return_ FLeX.notify_addr_ ; { _ } }} . 
+ Defined . 
+ 
+ (*begin*) 
+ Definition FLeX_Ф_getNotifyAddr_call  := 
+ 🏓 ursus_call_with_args ( LedgerableWithArgs := λ0 ) FLeX_Ф_getNotifyAddr 
+ . 
+ Notation " 'FLeX_Ф_getNotifyAddr_ref_' '(' ')' " := 
+ ( URResult ( FLeX_Ф_getNotifyAddr_call 
+ )) 
+ (in custom URValue at level 0 ) : ursus_scope . 
+ (*end*) 
+ 
+ Definition FLeX_Ф__fallback ( cell : ( ) : UExpression XInteger false . 
+ 	 	 refine {{ cell : ( ( ) @ "cell" ; { _ } }} . 
+ 	 	 refine {{ return_ 0 ; { _ } }} . 
+ Defined . 
+ 
+ (*begin*) 
+ Definition FLeX_Ф__fallback_call  ( cell : URValue (P false ) := 
+ 🏓 ursus_call_with_args ( LedgerableWithArgs := λ1 ) FLeX_Ф__fallback 
+ ( SimpleLedgerableArg URValue {{ Λ "cell" }} cell ) 
+ . 
+ Notation " 'FLeX_Ф__fallback_ref_' '(' cell ')' " := 
+ ( URResult ( FLeX_Ф__fallback_call 
+ cell )) 
+ (in custom URValue at level 0 , cell custom URValue at level 0 ) : ursus_scope . 
+ (*end*) 
+  *)
+
+End FLeXFuncs .
